Add `PUSH N` bytecode
This also adds more examples.  I think perhaps the next step is to
construct a more useful EVM interface.  This should have direct methods
for pushing and popping to the stack, along with those for writing to
memory, etc.

src/LeanEVM/Bytecode.lean
@@ -15,6 +15,9 @@ def eval_add (evm: EVM) : Outcome :=
   | [_] => Error StackUnderflow
   | [] => Error StackUnderflow
 
+def eval_push (evm: EVM)(n:u256) : Outcome :=
+  Ok {stack:=n::evm.stack}
+
 def eval_pop (evm: EVM) : Outcome :=
   match evm.stack with
   | _::rest => Ok { stack := rest }
@@ -26,17 +29,18 @@ def eval_dup (evm: EVM) : Outcome :=
   | [] => Error StackUnderflow
 
 -- Execute a given bytecodes from a given state.
-def eval (evm: EVM) : Bytecode -> Outcome
+@[simp] def eval (evm: EVM) : Bytecode -> Outcome
 | Bytecode.STOP => eval_stop evm
 | Bytecode.ADD => eval_add evm
 | Bytecode.POP => eval_pop evm
 | Bytecode.DUP => eval_dup evm
+| Bytecode.PUSH n => eval_push evm n
 
 -- Execute a sequence of zero or more bytecodes from a given state.
-def eval_all (code: List Bytecode)(evm:EVM) : Outcome :=
+@[simp] def eval_all (code: List Bytecode)(evm:EVM) : Outcome :=
   reduce code (Ok evm)
 where
-   reduce : (List Bytecode) -> Outcome -> Outcome
+   @[simp] reduce : (List Bytecode) -> Outcome -> Outcome
     | _,(Error err) => Error err
     | _,(Done gas data) => Done gas data
     | [],(Ok evm) => Ok evm
@@ -54,16 +58,30 @@ by
 -- Executing ADD on an empty EVM produces a stack overflow.
 example : (eval_all [ADD] EmptyEVM) = (Error StackUnderflow) :=
 by
-  unfold eval_all eval_all.reduce eval_all.reduce
-  unfold eval eval_add
-  unfold EmptyEVM
   simp
 
+-- Executing ADD on EVM with two operands succeeds.
+example (st:List u256): exists evm, (eval_all [ADD] {stack:=l::r::st}) = (Ok evm) :=
+by
+  exists {stack := (Fin.add l r)::st}
 
+-- Executing POP on EVM with at least one operand succeeds.
+example (st:List u256)(p:st = v::rest): (eval_all [POP] {stack:=st}) = (Ok {stack:=rest}) :=
+by
+  simp [p]
 
+-- Executing PUSH then POP on an EVM is a no-op.
+example (evm:EVM): (eval_all [PUSH n,POP] evm) = Ok evm :=
+by
+  simp
 
+-- Executing PUSH, PUSH, ADD on an EVM always succeeds.
+example (evm:EVM): ∃nevm, (eval_all [PUSH N, PUSH m, ADD] evm) = Ok nevm :=
+by
+  simp
 
-
-
-
-
+def list_dec (l:List u256)(p:l.length > 0) : exists h, exists t, l = h::t :=
+by
+  match l with
+  | h::t => exists h,t
+  | [] => contradiction
